lib/binaryTree.dfy
@@ -1,0 +1,235 @@
+include "../lib/seq.dfy"
+import opened Seq
+
+datatype Tree = Node(val: int, left: Tree, right: Tree) | Nil
+
+function method TreePreorderTraversal(root: Tree): seq<Tree>
+    // ensures forall x :: x in TreePreorderTraversal(root) ==> x != Nil
+    // ensures forall x :: x in TreePreorderTraversal(root) ==> x != Nil && (x == root || x in TreePreorderTraversal(root.left) || x in TreePreorderTraversal(root.right))
+    // ensures forall x :: x in root.repr ==> x in PreorderTraversal(root)
+    // ensures injectiveSeq(TreePreorderTraversal(root))
+    // ensures forall k :: 0 <= k < |TreePreorderTraversal(root)| ==> TreePreorderTraversal(root)[k] in root.repr
+    // ensures forall k :: 0 <= k < |PreorderTraversal(root)| ==> forall child :: child in PreorderTraversal(root)[k].repr && child != child in PreorderTraversal(root)[k] ==> exists j :: k < j < |PreorderTraversal(root)| && PreorderTraversal(root)[j] == child
+{
+   if root == Nil then [] else if root.left != Nil && root.right != Nil then [root]+TreePreorderTraversal(root.left)+TreePreorderTraversal(root.right) else if root.left != Nil then [root]+TreePreorderTraversal(root.left) else if root.right != Nil then [root]+TreePreorderTraversal(root.right) else [root]
+}
+
+predicate validTree(root: Tree) {
+    if root != Nil then root.left != root && root.right != root && (forall lchild :: lchild in TreePreorderTraversal(root.left) ==> lchild != root && lchild !in TreePreorderTraversal(root.right)) && (forall rchild :: rchild in TreePreorderTraversal(root.right) ==> rchild != root && rchild !in TreePreorderTraversal(root.left)) && validTree(root.right) && validTree(root.left) else true
+    // if root != Nil then root.left != root && root.right != root && root !in TreePreorderTraversal(root.left)  && root !in TreePreorderTraversal(root.right) && forall x :: x in TreePreorderTraversal(root.left) ==> x !in TreePreorderTraversal(root.right) && forall x :: x in TreePreorderTraversal(root.right) ==> x !in TreePreorderTraversal(root.left) && validTree(root.right) && validTree(root.left) else true
+}
+
+lemma rootNotInChildren(root: Tree)
+    requires root != Nil
+    requires validTree(root);
+    ensures root != Nil && root.left != Nil ==> root !in TreePreorderTraversal(root.left)
+    ensures root != Nil && root.right != Nil ==> root !in TreePreorderTraversal(root.right)
+{
+    assert root in TreePreorderTraversal(root);
+    tpt(root);
+    if root != Nil && root.left != Nil && root.right != Nil {
+        calc {
+            TreePreorderTraversal(root);
+            [root]+TreePreorderTraversal(root.left)+TreePreorderTraversal(root.right);
+        }
+        assert root !in TreePreorderTraversal(root.left);
+    }else{
+
+    }
+}
+
+lemma {:verify } TPTInjective(root: Tree) 
+    requires validTree(root)
+    requires root != Nil
+    ensures injectiveSeq(TreePreorderTraversal(root))
+{
+    NoNil(root);
+    tpt(root);
+    assert root !in TreePreorderTraversal(root.left);
+    assert root !in TreePreorderTraversal(root.right);
+    if root.right != Nil && root.left != Nil {
+        calc{
+            TreePreorderTraversal(root);
+            [root]+TreePreorderTraversal(root.left)+TreePreorderTraversal(root.right);
+        }
+        TPTInjective(root.left);
+        TPTInjective(root.right);
+        injectiveSeqs([root], TreePreorderTraversal(root.left));
+        injectiveSeqs([root] + TreePreorderTraversal(root.left), TreePreorderTraversal(root.right));
+
+    }else if root.right != Nil {
+        calc{
+            TreePreorderTraversal(root);
+            [root]+TreePreorderTraversal(root.right);
+        }
+        TPTInjective(root.right);
+        injectiveSeqs([root], TreePreorderTraversal(root.right));
+    }else if root.left != Nil {
+
+        calc{
+            TreePreorderTraversal(root);
+            [root]+TreePreorderTraversal(root.left);
+        }
+        TPTInjective(root.left);
+        injectiveSeqs([root], TreePreorderTraversal(root.left));
+    }
+}
+
+lemma NoNil(root: Tree)
+    ensures forall x :: x in TreePreorderTraversal(root) ==> x != Nil
+{
+
+}
+
+lemma tpt(root: Tree)
+    ensures forall x :: x in TreePreorderTraversal(root) ==> x != Nil
+    ensures forall x :: x in TreePreorderTraversal(root) ==> x != Nil && (x == root || x in TreePreorderTraversal(root.left) || x in TreePreorderTraversal(root.right))
+{
+
+}
+
+
+lemma AllChildTraversalElementsInRoot(root: Tree, elem: Tree)
+    requires elem in TreePreorderTraversal(root)
+    ensures forall child :: child in TreePreorderTraversal(elem) ==> child in TreePreorderTraversal(root)
+{
+
+}
+
+lemma TreePreorderTraversalSubstrings(root: Tree)
+    requires root != Nil
+    ensures root.left != Nil ==> isSubstring(TreePreorderTraversal(root.left), TreePreorderTraversal(root))
+    ensures root.right != Nil ==> isSubstring(TreePreorderTraversal(root.right), TreePreorderTraversal(root))
+{
+   if root.left != Nil && root.right != Nil {
+    calc {
+        TreePreorderTraversal(root);
+        [root]+TreePreorderTraversal(root.left)+TreePreorderTraversal(root.right);
+    }
+    var k := 1;
+    var j := |TreePreorderTraversal(root.left)|+1;
+    assert 0 <= k <= j <= |TreePreorderTraversal(root)| && TreePreorderTraversal(root.left) == TreePreorderTraversal(root)[1..|TreePreorderTraversal(root.left)|+1];
+
+    var s := 1+|TreePreorderTraversal(root.left)|;
+    var t := |TreePreorderTraversal(root)|;
+    assert 0 <= s <= t <= |TreePreorderTraversal(root)| && TreePreorderTraversal(root.right) == TreePreorderTraversal(root)[s..t];
+   }else if root.left != Nil && root.right == Nil {
+    calc {
+        TreePreorderTraversal(root);
+        [root]+TreePreorderTraversal(root.left);
+    }
+    var k := 1;
+    var j := |TreePreorderTraversal(root.left)|+1;
+    assert 0 <= k <= j <= |TreePreorderTraversal(root)| && TreePreorderTraversal(root.left) == TreePreorderTraversal(root)[1..j];
+   }else if root.left == Nil && root.right != Nil {
+    calc {
+        TreePreorderTraversal(root);
+        [root]+TreePreorderTraversal(root.right);
+    }
+    var k := 1;
+    var j := |TreePreorderTraversal(root.right)|+1;
+    assert 0 <= k <= j <= |TreePreorderTraversal(root)| && TreePreorderTraversal(root.right) == TreePreorderTraversal(root)[1..j];
+   }
+}
+
+lemma AllContained(root: Tree)
+    requires root != Nil
+    ensures forall x :: x in TreePreorderTraversal(root) ==> (x == root || x in TreePreorderTraversal(root.left) || x in TreePreorderTraversal(root.right))
+{
+}
+
+lemma {:verify true} {:induction false} AllChildrenTraversalsAreSubstrings(root: Tree) 
+    requires root != Nil
+    ensures forall x ::x in TreePreorderTraversal(root) ==> isSubstring(TreePreorderTraversal(x), TreePreorderTraversal(root))
+{
+    NoNil(root);
+    AllContained(root);
+    forall x | x in TreePreorderTraversal(root) 
+        ensures isSubstring(TreePreorderTraversal(x), TreePreorderTraversal(root))
+    {
+        tpt(root);
+        if x == root {
+            var k, j := 0, |TreePreorderTraversal(root)|;
+            assert 0 <= k <= j <= |TreePreorderTraversal(root)| && TreePreorderTraversal(root) == TreePreorderTraversal(root)[k..j];
+        }else if x == root.left || x == root.right {
+           TreePreorderTraversalSubstrings(root); 
+        }else {
+            if root.left != Nil && root.right != Nil {
+                assert x != root;
+                assert TreePreorderTraversal(root) == [root] + TreePreorderTraversal(root.left) + TreePreorderTraversal(root.right);
+                if root.left != Nil  && x in TreePreorderTraversal(root.left) {
+                    AllChildrenTraversalsAreSubstrings(root.left);
+                    assert isSubstring(TreePreorderTraversal(x), TreePreorderTraversal(root.left));
+                    TreePreorderTraversalSubstrings(root);
+                    AllSubstringsAreSubstrings(TreePreorderTraversal(x), TreePreorderTraversal(root.left), TreePreorderTraversal(root));
+                }
+                if root.right != Nil && x in TreePreorderTraversal(root.right) {
+                    AllChildrenTraversalsAreSubstrings(root.right);
+                    assert isSubstring(TreePreorderTraversal(x), TreePreorderTraversal(root.right));
+                    TreePreorderTraversalSubstrings(root);
+                    AllSubstringsAreSubstrings(TreePreorderTraversal(x), TreePreorderTraversal(root.right), TreePreorderTraversal(root));
+                }
+            }else if root.left != Nil  && x in TreePreorderTraversal(root.left) {
+                AllChildrenTraversalsAreSubstrings(root.left);
+                assert isSubstring(TreePreorderTraversal(x), TreePreorderTraversal(root.left));
+                    TreePreorderTraversalSubstrings(root);
+                    AllSubstringsAreSubstrings(TreePreorderTraversal(x), TreePreorderTraversal(root.left), TreePreorderTraversal(root));
+            }else  if root.right != Nil && x in TreePreorderTraversal(root.right) {
+                AllChildrenTraversalsAreSubstrings(root.right);
+                    assert isSubstring(TreePreorderTraversal(x), TreePreorderTraversal(root.right));
+                    TreePreorderTraversalSubstrings(root);
+                    AllSubstringsAreSubstrings(TreePreorderTraversal(x), TreePreorderTraversal(root.right), TreePreorderTraversal(root));
+            }else{
+                assert x != root;
+                assert x !in TreePreorderTraversal(root.left);
+                assert x !in TreePreorderTraversal(root.right);
+                assert false;
+            }
+        }
+    }
+}
+
+lemma TreeChildrenAreLater(root: Tree)
+    requires root != Nil
+    ensures forall x :: x in TreePreorderTraversal(root) && x != root ==> exists k:nat :: 0 < k < |TreePreorderTraversal(root)| && TreePreorderTraversal(root)[k] == x
+{
+    NoNil(root);
+}
+
+lemma {:verify true} TreePreorderTraversalChildrenAreLater3(root: Tree, elem: Tree, k: nat) 
+    // requires validTree(root)
+    requires injectiveSeq(TreePreorderTraversal(root))
+    requires k < |TreePreorderTraversal(root)|
+    requires elem in TreePreorderTraversal(root)
+    requires elem != Nil
+    requires TreePreorderTraversal(root)[k] == elem
+    ensures forall child :: child in TreePreorderTraversal(elem) && child != elem ==> exists j: nat :: k < j < |TreePreorderTraversal(root)| && TreePreorderTraversal(root)[j] == child
+{
+    // TPTInjective(root);
+    AllChildTraversalElementsInRoot(root, elem);
+    AllChildrenTraversalsAreSubstrings(root);
+    AllChildrenTraversalsAreSubstrings(elem);
+    TreeChildrenAreLater(elem);
+    forall child | child in TreePreorderTraversal(elem) && child != elem
+        ensures exists j: nat :: k < j < |TreePreorderTraversal(root)| && TreePreorderTraversal(root)[j] == child
+    {
+        assert child in TreePreorderTraversal(root);
+        assert child != elem;
+        var j:nat :| 0 < j < |TreePreorderTraversal(elem)| && TreePreorderTraversal(elem)[j] == child;
+        var s,t :| 0 <= s < t <= |TreePreorderTraversal(root)| && TreePreorderTraversal(elem) == TreePreorderTraversal(root)[s..t];
+        assert TreePreorderTraversal(root)[k] == elem;
+        assert TreePreorderTraversal(elem)[0] == elem;
+        assert TreePreorderTraversal(root)[s] == elem;
+        assert s == k;
+        assert TreePreorderTraversal(root)[s+j] == child;
+
+        // seqbusiness(TreePreorderTraversal(root), child);
+        // var j :| 0 <= j < |TreePreorderTraversal(root)| && TreePreorderTraversal(root)[j] == child;
+        // assert isSubstring(TreePreorderTraversal(child), TreePreorderTraversal(elem));
+        // AllSubstringsAreSubstrings(TreePreorderTraversal(child), TreePreorderTraversal(elem), TreePreorderTraversal(root));
+        // assert isSubstring(TreePreorderTraversal(child), TreePreorderTraversal(root));
+        // // assert |TreePreorderTraversal(child)| <= |TreePreorderTraversal(elem)|;
+        // var s,t :| 0 <= s < t <= |TreePreorderTraversal(root)| && TreePreorderTraversal(child) == TreePreorderTraversal(root)[s..t];
+        // assert j == s;
+    }
+}
